
## 求和公式

$$
\sum_{i}^{n}{i} = \frac{n(n+1)}{2}
$$

$$
\sum_{i}^{n}{i}^2 = \frac{n(n+1)(2n+1)}{6}
$$

## 求导公式

$$
{f}'{(x)} = \frac{\mathrm{d} y}{\mathrm{d} x} 
$$


$$
\Delta{x} = \mathrm{d} x
$$

$$
\Delta{\mathrm{d} y} = \mathrm{\mathrm{d} y} +  o {(\Delta{x})} 
$$

$$
\lim_{x \to 0} {\mathrm{d} y} = 0
$$

$$
\lim_{x \to 0} {\mathrm{d} x} = 0
$$

### 一阶求导

$$
{C}' = 0
$$

$$
{({a}^{n})}' =  n \cdot{a}^{n-1}
$$


### 幂运算

$$a^m\cdot a^n\cdot a^p = a^{a+m+p}$$

$$(a^{m})^{n}=a^{mn}$$

$$\frac{a^{m}}{a^{n}}=a^{m-n}$$

$$a^0=1 (a \ne 0)$$

$$
x^n=a => x=a^{\frac{1}{n}}
$$
$$a^{-n}=\frac{1}{a^{n}} (a\ne 0)$$